Mica/SeparationLogic/Axioms.lean
@@ -43,12 +43,6 @@ axiom wp.bind {k : TinyML.K} {e : Runtime.Expr} {Q : Runtime.Val → iProp} :
 axiom wp.mono {e : Runtime.Expr} {P Q : Runtime.Val → iProp} :
     (∀ v, P v -∗ Q v) ∗ wp e P ⊢ wp e Q
 
-axiom wp.fix {f : Runtime.Binder} {args : List Runtime.Binder} {e : Runtime.Expr}
-    {P : Runtime.Val → iProp} {Φ : List Runtime.Val → iProp} :
-    ((∀ vs, Φ vs -∗ wp (.app (.val (.fix f args e)) (vs.map Runtime.Expr.val)) P) -∗
-      ∀ vs, Φ vs -∗ wp (e.subst ((Runtime.Subst.id.update' f (.fix f args e)).updateAll' args vs)) P)
-    ⊢ (∀ (vs : List Runtime.Val), Φ vs -∗ wp (.app (.val (.fix f args e)) (vs.map Runtime.Expr.val)) P)
-
 axiom wp.app {fn : Runtime.Expr} {args : Runtime.Exprs} {P : Runtime.Val → iProp} :
     wps args (fun vs => wp fn (fun fv =>
       wp (.app (.val fv) (vs.map Runtime.Expr.val)) P)) ⊢
@@ -58,15 +52,18 @@ axiom wp.func {f : Runtime.Binder} {args : List Runtime.Binder} {e : Runtime.Exp
     (P : Runtime.Val → iProp) :
     P (.fix f args e) ⊢ wp (.fix f args e) P
 
--- @agent: wp.fix' needs several persistency modalities that are currently missing
+axiom wp.fix {f : Runtime.Binder} {args : List Runtime.Binder} {e : Runtime.Expr}
+    {P : Runtime.Val → iProp} {Φ : List Runtime.Val → iProp} :
+      wp (e.subst ((Runtime.Subst.id.update' f (.fix f args e)).updateAll' args vs)) P
+    ⊢ wp (.app (.val (.fix f args e)) (vs.map Runtime.Expr.val)) P
+
 axiom wp.fix' {f : Runtime.Binder} {args : List Runtime.Binder} {e : Runtime.Expr}
     {Φ : (Runtime.Val → iProp) → List Runtime.Val → iProp} :
-    ((∀ (vs : List Runtime.Val) (P : Runtime.Val → iProp),
+    □ (□ (∀ (vs : List Runtime.Val) (P : Runtime.Val → iProp),
         Φ P vs -∗ wp (.app (.val (.fix f args e)) (vs.map Runtime.Expr.val)) P) -∗
       ∀ (vs : List Runtime.Val) (P : Runtime.Val → iProp),
         Φ P vs -∗ wp (e.subst ((Runtime.Subst.id.update' f (.fix f args e)).updateAll' args vs)) P)
-    ⊢ (∀ (vs : List Runtime.Val) (P : Runtime.Val → iProp),
-        Φ P vs -∗ wp (.app (.val (.fix f args e)) (vs.map Runtime.Expr.val)) P)
+    ⊢ □ (∀ (vs : List Runtime.Val) (P : Runtime.Val → iProp), Φ P vs -∗ wp (.app (.val (.fix f args e)) (vs.map Runtime.Expr.val)) P)
 
 axiom wp.unop {op : TinyML.UnOp} {v res : Runtime.Val} {Q : Runtime.Val → iProp} :
     TinyML.evalUnOp op v = some res →
